untracked trait changes

case_studies/tests/src/traits.rs
@@ -54,9 +54,64 @@ fn test_add_2<T>(x: T, y: T) where T: MyAdd {
     //let _bla = x.bla();
 //}
 
+/*
+trait XX {
+
+}
+
+trait Foo<T> where Self: XX {
+    type Output;
+    
+    #[rr::params("a", "b")]
+    #[rr::args("#a", "b")]
+    #[rr::exists("y")]
+    #[rr::returns("y")]
+    fn bar<U> (&self, x: U) -> (Self::Output, T, U);
+}
+
+impl XX for i32 {
+
+}
+
+impl Foo<u32> for i32 {
+    
+    type Output = i32;
+    
+    #[rr::params("a", "b")]
+    #[rr::args("#a", "b")]
+    #[rr::exists("y")]
+    #[rr::returns("y")]
+    fn bar<U> (&self, x: U) -> (i32, u32, U) {
+        ( *self, 42, x)
+    }
+}
+
+#[rr::params("w")]
+#[rr::args("#w")]
+fn foobar2<W, T> (x: &W) where W: Foo<T> {
+    // NOTE: for this, we need to look up the Alias type in the trait registry.
+    x.bar(true);
+}
+
+#[rr::returns("()")]
+fn call_foobar2() {
+    let a = 0;
+    foobar2(&a);
+}
+*/
+
+// Note: this is invalid!
+/*
+trait FooB<T> 
+    where Self : FooB<T>
+{
+    type Output;
+}
+*/
 
 
-trait Foo<T> {
+trait Foo<T> 
+{
     type Output;
     
     #[rr::params("a", "b")]
@@ -76,6 +131,18 @@ impl Foo<u32> for i32 {
     #[rr::returns("y")]
     fn bar<U> (&self, x: U) -> (i32, u32, U) {
         ( *self, 42, x)
+    }
+}
+
+// So, I can also do requirements which might only be fulfilled later.
+// (i.e. the requirement on T might be fulfilled by another instance).
+impl<T> Foo<i32> for T 
+    where T : Foo<i32>
+{
+    type Output = i32;
+
+    fn bar<U>(&self, x : U ) -> (Self::Output, i32, U) {
+        unimplemented!();
     }
 }
 
