rr_frontend/translation/src/trait_registry.rs
@@ -1,5 +1,5 @@
 use std::cell::RefCell;
-use std::collections::HashMap;
+use std::collections::{HashSet, HashMap};
 
 use log::{info, trace};
 use radium::{code, specs};
@@ -9,18 +9,22 @@ use typed_arena::Arena;
 
 use crate::base::TranslationError;
 use crate::environment::Environment;
-use crate::type_translator::{InFunctionState, generate_args_inst_key, GenericsKey, TypeTranslator, LocalTypeTranslator, strip_coq_ident};
-
-use crate::utils;
-use crate::function_body::{get_arg_syntypes_for_procedure_call, FunctionTranslator, mangle_name_with_args};
-
+use crate::function_body::{get_arg_syntypes_for_procedure_call, mangle_name_with_args, FunctionTranslator};
 use crate::spec_parsers::propagate_method_attr_from_impl;
+use crate::type_translator::{
+    generate_args_inst_key, strip_coq_ident, GenericsKey, InFunctionState, LocalTypeTranslator,
+    TypeTranslator,
+};
+use crate::utils;
 
+use derive_more::Constructor;
 
 #[derive(Debug, Clone)]
 pub enum TraitRegistryError<'tcx> {
     /// This DefId is not a trait
     NotATrait(DefId),
+    /// This DefId is not an impl of a trait
+    NotATraitImpl(DefId),
     /// This DefId is not a trait method
     NotATraitMethod(DefId),
     /// This DefId is not an assoc type
@@ -36,153 +40,6 @@ pub enum TraitRegistryError<'tcx> {
 }
 pub type TraitRegistryResult<'tcx, T> = Result<T, TraitRegistryError<'tcx>>;
 
-
-/// Get the name of a trait method without the path prefix.
-pub fn get_assoc_item_name<'tcx>(tcx: ty::TyCtxt<'tcx>, trait_method_did: DefId) -> Option<String> {
-    let def_path = tcx.def_path(trait_method_did);
-    if let Some(last_elem) = def_path.data.last() {
-        if let Some(name) = last_elem.data.get_opt_name() {
-            return Some(strip_coq_ident(name.as_str()));
-        }
-    }
-    None
-}
-
-/// A specification for a particular instance of a trait
-#[derive(Clone, Debug)]
-pub struct TraitInstanceSpec<'def> {
-    /// a map from identifiers to the associated types
-    assoc_types: HashMap<String, specs::LiteralTyParam>,
-    /// a map from the identifiers to the method specs
-    methods: HashMap<String, specs::FunctionSpec<'def>>,
-}
-
-/// A using occurrence of a trait spec.
-#[derive(Debug, Clone)]
-pub struct LiteralTraitSpec {
-    /// Name of the trait
-    pub name: String,
-
-    /// The name of the Coq definition for the spec information
-    /// (Coq def has no parameter)
-    pub spec_record: String,
-
-    /// The basic specification annotated on the trait definition
-    /// (Coq def has self, type parameters, as well as associated types)
-    pub base_spec: String,
-    /// The subsumption relation between specs
-    /// (Coq def has no parameters)
-    pub spec_subsumption: String,
-}
-pub type LiteralTraitSpecRef<'def> = &'def LiteralTraitSpec;
-
-impl LiteralTraitSpec {
-    /// Make the name for the method spec field of the spec record.
-    pub fn make_spec_method_name(&self, method: &str) -> String {
-        format!("{}_{method}_spec", self.name)
-    }
-}
-
-/// A reference to a trait instantiated with its parameters in the verification of a function.
-#[derive(Debug, Clone)]
-pub struct LiteralTraitSpecUse<'def> {
-    pub trait_ref: LiteralTraitSpecRef<'def>,
-    /// the instantiation for the self parameter
-    pub self_inst: specs::Type<'def>,
-    /// the instantiation for the type parameters
-    pub params_inst: Vec<specs::Type<'def>>,
-
-    /// the name including the generic args
-    mangled_base: String,
-}
-
-impl<'def> LiteralTraitSpecUse<'def> {
-    pub fn new(
-        trait_ref: LiteralTraitSpecRef<'def>,
-        self_inst: specs::Type<'def>,
-        params_inst: Vec<specs::Type<'def>>,
-        mangled_base: String,
-    ) -> Self {
-        Self {
-            trait_ref,
-            self_inst,
-            params_inst,
-            mangled_base,
-        }
-    }
-
-    /// Get the name for a spec parameter for this trait instance.
-    pub fn make_spec_param_name(&self) -> String {
-        format!("{}_spec", self.mangled_base)
-    }
-
-    /// Make the name for the location parameter of a use of a method of this trait parameter.
-    pub fn make_loc_name(&self, mangled_method_name: &str) -> String {
-        format!("{}_{}_loc", self.mangled_base, mangled_method_name)
-    }
-
-    /// Make the term for the specification of the given method.
-    pub fn make_method_spec_term(&self, method_name: &str) -> String {
-        format!("{}.({})", self.make_spec_param_name(), self.trait_ref.make_spec_method_name(method_name))
-    }
-
-    /// Make the names for the Coq-level parameters for an associated type of this instance.
-    pub fn make_assoc_type_lit(&self, assoc_type: &str) -> specs::LiteralTyParam {
-        let rust_name = format!("{}_{}", self.mangled_base, assoc_type);
-        let ty_name = format!("{rust_name}_ty");
-        let rt_name = format!("{rust_name}_rt");
-        let st_name = format!("{rust_name}_st");
-
-        specs::LiteralTyParam {
-            rust_name,
-            type_term: ty_name,
-            refinement_type: rt_name, 
-            syn_type: st_name,
-        }
-    }
-}
-
-/// When translating a trait declaration, we should generate this, bundling all the components of
-/// the trait together.
-#[derive(Clone, Debug)]
-pub struct TraitSpecDecl<'def> {
-    /// A reference to all the Coq definition names we should generate.
-    pub lit: LiteralTraitSpecRef<'def>,
-
-    /// a list of extra things we assume in the Coq context
-    extra_coq_context: specs::CoqParamList,
-
-    /// The generics this trait uses
-    generics: Vec<Option<specs::LiteralTyParam>>,
-
-    /// The default specification from the trait declaration
-    default_spec: TraitInstanceSpec<'def>,
-}
-
-impl<'def> TraitSpecDecl<'def> {
-    //pub fn new(lit: LiteralTraitSpecRef<'def>, extra_params
-}
-
-/// When translating an impl block, we should generate this, which bundles all components of the
-/// implementation together.
-pub struct ImplSpec<'def> {
-    /// name of the implementation
-    name: String,
-    /// The name of the record instance for physical information
-    phys_record: String,
-    /// The name of the record instance for spec information
-    spec_record: String,
-    /// The name of the proof that the base spec is implied by the more specific spec
-    spec_subsumption: String,
-
-    /// reference to the trait this is implementing
-    of_trait: LiteralTraitSpecRef<'def>,
-
-    /// the implementation of the associated types
-    assoc_types: HashMap<String, specs::Type<'def>>,
-    /// the implementation and specification for the method implementations
-    methods: HashMap<String, code::Function<'def>>,
-}
 
 /// What does a trait registry need?
 ///
@@ -230,17 +87,21 @@ pub struct TraitRegistry<'tcx, 'def> {
     type_translator: &'def TypeTranslator<'def, 'tcx>,
 
     /// trait declarations
-    trait_decls: RefCell<HashMap<LocalDefId, TraitSpecDecl<'def>>>,
+    trait_decls: RefCell<HashMap<LocalDefId, specs::TraitSpecDecl<'def>>>,
     /// trait literals for using occurrences, including shims we import
-    trait_literals: RefCell<HashMap<DefId, LiteralTraitSpecRef<'def>>>,
+    trait_literals: RefCell<HashMap<DefId, specs::LiteralTraitSpecRef<'def>>>,
 
     /// arena for allocating trait literals
-    trait_arena: &'def Arena<LiteralTraitSpec>,
+    trait_arena: &'def Arena<specs::LiteralTraitSpec>,
 }
 
 impl<'tcx, 'def> TraitRegistry<'tcx, 'def> {
     /// Create an empty trait registry.
-    pub fn new(env: &'def Environment<'tcx>, ty_translator: &'def TypeTranslator<'def, 'tcx>, arena: &'def Arena<LiteralTraitSpec>) -> Self {
+    pub fn new(
+        env: &'def Environment<'tcx>,
+        ty_translator: &'def TypeTranslator<'def, 'tcx>,
+        arena: &'def Arena<specs::LiteralTraitSpec>,
+    ) -> Self {
         Self {
             env,
             type_translator: ty_translator,
@@ -251,19 +112,45 @@ impl<'tcx, 'def> TraitRegistry<'tcx, 'def> {
     }
 
     /// Get registered trait declarations in the local crate.
-    pub fn get_trait_decls(&self) -> HashMap<LocalDefId, TraitSpecDecl<'def>> {
-        let decls = self.trait_decls.borrow();     
+    pub fn get_trait_decls(&self) -> HashMap<LocalDefId, specs::TraitSpecDecl<'def>> {
+        let decls = self.trait_decls.borrow();
         decls.clone()
     }
 
+    /// Get a map of dependencies between traits.
+    pub fn get_trait_deps(&self) -> HashMap<DefId, HashSet<DefId>> {
+        let mut dep_map = HashMap::new();
+
+        let decls = self.trait_decls.borrow();
+        for trait_decl in decls.keys() {
+            // check for other traits we need
+            let param_env: ty::ParamEnv<'tcx> = self.env.tcx().param_env(trait_decl.to_def_id());
+
+            let mut deps = HashSet::new();
+            for clause in param_env.caller_bounds() {
+                let kind = clause.kind().skip_binder();
+                if let ty::ClauseKind::Trait(pred) = kind {
+                    let other_did = pred.trait_ref.def_id;
+
+                    if other_did != trait_decl.to_def_id() {
+                        deps.insert(other_did);
+                    }
+                }
+            }
+            dep_map.insert(trait_decl.to_def_id(), deps);
+        }
+
+        dep_map
+    }
+
     /// Generate names for a trait.
-    fn make_literal_trait_spec(name: String) -> LiteralTraitSpec {
+    fn make_literal_trait_spec(name: String) -> specs::LiteralTraitSpec {
         let phys_record = format!("{name}_phys");
         let spec_record = format!("{name}_spec");
         let base_spec = format!("{name}_base_spec");
         let spec_subsumption = format!("{name}_spec_incl");
 
-        LiteralTraitSpec {
+        specs::LiteralTraitSpec {
             name,
             spec_record,
             base_spec,
@@ -272,42 +159,94 @@ impl<'tcx, 'def> TraitRegistry<'tcx, 'def> {
     }
 
     /// Register a new annotated trait in the local crate with the registry.
-    pub fn register_trait(&self, did: LocalDefId) -> TraitRegistryResult<'tcx, ()> {
+    pub fn register_trait(&'def self, ty_translator: &'def TypeTranslator<'def, 'tcx>, did: LocalDefId) -> Result<(), TranslationError<'tcx>> {
         trace!("enter TraitRegistry::register_trait for did={did:?}");
+
+        {
+            let scope = self.trait_decls.borrow();
+            if scope.get(&did).is_some() {
+                return Ok(());
+            }
+        }
+
+        // TODO: can we handle the case that this depends on a generic having the same trait? 
+        // In principle, yes, but currently the implementation does not allow it.
+        // We also do not generate trait dep parameters. 
+        // We should depend on the assoc types of the other traits as well as the specs.
 
         // make the literal we are going to use
         let trait_name = strip_coq_ident(&self.env.get_absolute_item_name(did.to_def_id()));
-        let lit_trait_spec = Self::make_literal_trait_spec(trait_name);
-        // already register it for use
+        let lit_trait_spec = Self::make_literal_trait_spec(trait_name.clone());
+        // already register it for use.
+        // In particular, this is also needed to be able to register the methods of this trait
+        // below, as they need to be able to access the associated types of this trait already.
+        // (in fact, their environment contains their self instance)
         let lit_trait_spec_ref = self.register_shim(did.to_def_id(), lit_trait_spec)?;
 
         // get generics
-        // TODO
-
-        // get items
-        let children = self.env.tcx().module_children_local(did);
-        for c in children.iter() {
-            if let rustc_hir::def::Res::Def(def_kind, def_id) = c.res {
-                if def_kind == rustc_hir::def::DefKind::AssocFn {
-
-                    // get attributes
-                    let attrs = self.env.get_attributes_of_function(did.into(), |x| propagate_method_attr_from_impl(x));
-
-                    // get function name
-                    let name = get_assoc_item_name(self.env.tcx(), did.into()).ok_or_else(|| TraitRegistryError::NotATraitMethod(did.into()))?;
-
-                    // TODO
-                    //FunctionTranslator::spec_for_trait_method(&self.env, def_id, ) 
-                     
-                }
-
+        let trait_generics: &'tcx ty::Generics = self.env.tcx().generics_of(did.to_def_id());
+        let mut generic_env = Vec::new();
+        for param in trait_generics.params.iter() {
+            if let rustc_middle::ty::GenericParamDefKind::Type { .. } = param.kind {
+                let name = param.name.as_str();
+                let lit = specs::LiteralTyParam::new(&name, &name);
+                generic_env.push(Some(lit)); 
+            }
+            else {
+                generic_env.push(None);
             }
         }
-        
-        //let decl = TraitSpecDecl
+
+        // get extra context items from trait annotation
+        // TODO
+        let extra_context_items = Vec::new();
+        let extra_context_items = specs::CoqParamList(extra_context_items);
+
+        // get items
+        let mut methods = HashMap::new();
+        let mut assoc_types = Vec::new();
+        let items: &ty::AssocItems = self.env.tcx().associated_items(did);
+        for c in items.in_definition_order() {
+            if ty::AssocKind::Fn == c.kind {
+                // get attributes
+                let attrs =
+                    self.env.get_attributes_of_function(c.def_id, |x| propagate_method_attr_from_impl(x));
+
+                // get function name
+                let method_name = self
+                    .env
+                    .get_assoc_item_name(c.def_id)
+                    .ok_or(TraitRegistryError::NotATraitMethod(c.def_id))?;
+                let method_name = strip_coq_ident(&method_name);
+
+                let name = format!("{trait_name}_{method_name}");
+                let spec_name = format!("{name}_base_spec");
+
+                // get spec
+                let spec = FunctionTranslator::spec_for_trait_method(self.env, c.def_id, name.clone(), spec_name, attrs.as_slice(), ty_translator, &self)?;
+
+                methods.insert(method_name, spec); 
+            }
+            else if ty::AssocKind::Type == c.kind {
+                // get name
+                let type_name = self
+                    .env
+                    .get_assoc_item_name(c.def_id)
+                    .ok_or(TraitRegistryError::NotATraitMethod(c.def_id))?;
+                let type_name = strip_coq_ident(&type_name);
+                let lit = radium::LiteralTyParam::new(&type_name, &type_name);
+                assoc_types.push(lit);
+            }
+        }
+
+        let base_instance_spec = specs::TraitInstanceSpec::new(methods);
+        let decl = specs::TraitSpecDecl::new(lit_trait_spec_ref, extra_context_items, generic_env, assoc_types, base_instance_spec);
+
+        let mut scope = self.trait_decls.borrow_mut();
+        scope.insert(did, decl);
 
         trace!("leave TraitRegistry::register_trait");
-        Err(TraitRegistryError::Unknown)
+        Ok(())
     }
 
     /// Register a shim with the trait registry.
@@ -315,11 +254,11 @@ impl<'tcx, 'def> TraitRegistry<'tcx, 'def> {
     /// Errors:
     /// - NotATrait(did) if did is not a trait
     /// - TraitAlreadyExists(did) if this trait has already been registered
-    pub fn register_shim(
-        &self,
+    pub fn register_shim<'a>(
+        &'a self,
         did: DefId,
-        spec: LiteralTraitSpec,
-    ) -> TraitRegistryResult<'tcx, LiteralTraitSpecRef<'def>> {
+        spec: specs::LiteralTraitSpec,
+    ) -> TraitRegistryResult<'tcx, specs::LiteralTraitSpecRef<'def>> {
         if !self.env.tcx().is_trait(did) {
             return Err(TraitRegistryError::NotATrait(did));
         }
@@ -336,10 +275,90 @@ impl<'tcx, 'def> TraitRegistry<'tcx, 'def> {
     }
 
     /// Lookup a trait.
-    pub fn lookup_trait(&self, trait_did: DefId) -> Option<LiteralTraitSpecRef<'def>> {
+    pub fn lookup_trait(&self, trait_did: DefId) -> Option<specs::LiteralTraitSpecRef<'def>> {
         let trait_literals = self.trait_literals.borrow();
         trait_literals.get(&trait_did).copied()
     }
+
+    /// Get the term for the specification of a trait impl (applied to the given arguments of the trait), 
+    /// as well as the list of associated types.
+    pub fn get_impl_spec_term(&self, ty_translator: &LocalTypeTranslator<'def, 'tcx>, impl_did: DefId, impl_args: &[ty::GenericArg<'tcx>], trait_args: &[ty::GenericArg<'tcx>]) -> Result<(String, Vec<radium::Type<'def>>), TranslationError<'tcx>> {
+        trace!("enter TraitRegistry::get_impl_spec_term for impl_did={impl_did:?} impl_args={impl_args:?} trait_args={trait_args:?}");
+        let trait_did = self.env.tcx().trait_id_of_impl(impl_did).ok_or(TraitRegistryError::NotATraitImpl(impl_did))?;
+
+        let trait_instance = self.lookup_trait(trait_did).ok_or(TraitRegistryError::NotATrait(trait_did))?;
+
+        // the base_spec gets all the trait's args as well as the associated types
+        let mut all_trait_args = Vec::new();
+        for arg in trait_args.iter() {
+            if let ty::GenericArgKind::Type(ty) = arg.unpack() {
+                let ty = ty_translator.translate_type(&ty)?;
+                all_trait_args.push(ty);
+            }
+        }
+
+        let mut assoc_args = Vec::new();
+        // get associated types of this impl
+        let assoc_items: &'tcx ty::AssocItems = self.env.tcx().associated_items(impl_did);
+        for it in assoc_items.in_definition_order() {
+            if it.kind == ty::AssocKind::Type {
+                let item_did = it.def_id;
+                let item_ty: ty::EarlyBinder<ty::Ty<'tcx>> = self.env.tcx().type_of(item_did);
+                let subst_ty = item_ty.instantiate(self.env.tcx(), impl_args);
+
+                let translated_ty = ty_translator.translate_type(&subst_ty)?;
+                all_trait_args.push(translated_ty.clone());
+                assoc_args.push(translated_ty);
+            }
+        }
+
+        let term = specs::CoqAppTerm::new(trait_instance.base_spec.clone(), all_trait_args.iter().map(|x| x.to_string()).collect());
+
+        trace!("leave TraitRegistry::get_impl_spec_term");
+        Ok((term.to_string(), assoc_args))
+    }
+}
+
+
+/// Check if this is a built-in trait
+pub fn is_builtin_trait(tcx: ty::TyCtxt<'_>, trait_did: DefId) -> Option<bool> {
+    let sized_did = utils::try_resolve_did(tcx, &["core", "marker", "Sized"])?;
+
+    // TODO: for these, should instead require the primitive encoding of our Coq formalization
+    let send_did = utils::try_resolve_did(tcx, &["core", "marker", "Send"])?;
+    let sync_did = utils::try_resolve_did(tcx, &["core", "marker", "Sync"])?;
+    let copy_did = utils::try_resolve_did(tcx, &["core", "marker", "Copy"])?;
+
+    Some(trait_did == sized_did)
+}
+
+/// Get non-trivial trait requirements of a function's ParamEnv.
+pub fn get_nontrivial_trait_requirements<'tcx>(tcx: ty::TyCtxt<'tcx>, param_env: ty::ParamEnv<'tcx>) -> Vec<ty::TraitRef<'tcx>> {
+    let mut trait_refs = Vec::new();
+
+    // TODO: check if caller_bounds does the right thing for implied bounds
+    let clauses = param_env.caller_bounds(); 
+    for cl in clauses.iter() {
+        let cl_kind = cl.kind();
+        let cl_kind = cl_kind.skip_binder();
+
+        // only look for trait predicates for now
+        if let ty::ClauseKind::Trait(trait_pred) = cl_kind {
+            // We ignore negative polarities for now
+            if trait_pred.polarity == ty::ImplPolarity::Positive {
+                let trait_ref = trait_pred.trait_ref;
+
+                // filter Sized, Copy, Send, Sync?
+                if Some(true) == is_builtin_trait(tcx, trait_ref.def_id) {
+                    continue;
+                }
+
+                // this is a nontrivial requirement
+                trait_refs.push(trait_ref); 
+            }
+        }
+    }
+    trait_refs
 }
 
 /// A using occurrence of a trait in the signature of the function.
@@ -350,7 +369,7 @@ pub struct GenericTraitUse<'def> {
     /// the self type this is implemented for
     self_ty: ty::ParamTy,
     /// the Coq-level trait use
-    pub trait_use: LiteralTraitSpecUse<'def>,
+    pub trait_use: specs::LiteralTraitSpecUse<'def>,
 }
 
 impl<'def> GenericTraitUse<'def> {
@@ -359,7 +378,8 @@ impl<'def> GenericTraitUse<'def> {
         type_translator: &TypeTranslator<'def, 'tcx>,
         scope: InFunctionState<'_, 'def, 'tcx>,
         trait_ref: ty::TraitRef<'tcx>,
-        spec_ref: LiteralTraitSpecRef<'def>,
+        spec_ref: radium::LiteralTraitSpecRef<'def>,
+        is_used_in_self_trait: bool,
     ) -> Self {
         let did = trait_ref.def_id;
 
@@ -383,9 +403,13 @@ impl<'def> GenericTraitUse<'def> {
             unreachable!("self should be a Param");
         };
 
+        // TODO: allow to override the assumed specification using attributes
+        let spec_override = None;
+
         // create a name for this instance by including the args
         let mangled_base = mangle_name_with_args(&format!("{}", spec_ref.name), trait_ref.args.as_slice());
-        let spec_use = LiteralTraitSpecUse::new(spec_ref, translated_self, translated_args, mangled_base);
+        let spec_use =
+            specs::LiteralTraitSpecUse::new(spec_ref, translated_self, translated_args, mangled_base, spec_override, is_used_in_self_trait);
 
         Self {
             did,
@@ -393,10 +417,38 @@ impl<'def> GenericTraitUse<'def> {
             trait_use: spec_use,
         }
     }
+
+    /// Get the associated types we require for this trait use.
+    pub fn get_associated_type_literals(&self, env: &Environment<'_>) -> Vec<specs::LiteralTyParam> {
+        let mut assoc_tys: Vec<specs::LiteralTyParam> = Vec::new();
+
+        // get associated types
+        let assoc_types = env.get_trait_assoc_types(self.did);
+        for ty_did in assoc_types.iter() {
+            let ty_name = env.get_assoc_item_name(*ty_did).unwrap();
+            let lit = self.trait_use.make_assoc_type_lit(&strip_coq_ident(&ty_name));
+            assoc_tys.push(lit);
+        }
+        assoc_tys
+    }
 }
 
 // Next steps:
-// - implement lookup when calling a Param function
 // - add trait registration from code
-// - add trait shim generation
-// - add the trait requirements to the emitted code
+
+// Note: if I use a function which has traits, I need to provide it with the specification I provide.
+// This is something I have to provide as the caller
+// I need to look in the trait registry and check for registered instances
+// TODO: add notion of registered instances/ instance registry.
+//
+// I guess when I register that I call a function, I should check whether it requires any trait
+// implementations (i.e., go over its clauses)
+// I should then find out which instance will get picked for it, i.e. which instance gets picked.
+//  either this is a Param instance
+//  or it's an instance I can concretely resolve.
+// in the former case, I guess I give it the spec param recursively
+// in the latter case, I check if I have a registered spec for this instance, and use that.
+//
+// How about structs which use associated types?
+// if it's not statically resolvable, I guess it just acts as another type parameter, and it should
+// TODO: shelve ADTs with trait constraints
